

$$1. \quad m(a+bX) = \frac{1}{N} \sum_{i=1}^N a + bX_i = \frac{1}{N} \left( \sum_{i=1}^N a + b \sum_{i=1}^N X_i \right) = \frac{1}{N} \left( Na + b \sum_{i=1}^N X_i \right) \\ = a + b \left( \frac{1}{N} \sum_{i=1}^N X_i \right) = a + b m(X)$$

$$2. \quad \text{cov}(X, a+bY) = \frac{1}{N} \sum_{i=1}^N (X_i - m(X)) ((a+bY_i) - m(a+bY))$$

$$(a+bY_i) - m(a+bY) = b(Y_i - m(Y))$$

$$= \frac{1}{N} \sum_{i=1}^N (X_i - m(X)) \cdot b(Y_i - m(Y)) = b \left( \frac{1}{N} \sum_{i=1}^N (X_i - m(X))(Y_i - m(Y)) \right)$$

$$= b \text{cov}(X, Y)$$

~~$$3. \quad \text{cov}(a+bX, a+bX) = \frac{1}{N} \sum_{i=1}^N (Z_i - m(Z))^2$$~~